src/Compilers/Named/Context.v
@@ -5,14 +5,14 @@ Require Import Crypto.Util.Notations.
 
 Record Context {base_type_code} (Name : Type) (var : base_type_code -> Type) :=
   { ContextT : Type;
-    lookupb : ContextT -> Name -> forall {t : base_type_code}, option (var t);
-    extendb : ContextT -> Name -> forall {t : base_type_code}, var t -> ContextT;
-    removeb : ContextT -> Name -> base_type_code -> ContextT;
+    lookupb : forall {t : base_type_code}, ContextT -> Name -> option (var t);
+    extendb : forall {t : base_type_code}, ContextT -> Name -> var t -> ContextT;
+    removeb : base_type_code -> ContextT -> Name -> ContextT;
     empty : ContextT }.
 Coercion ContextT : Context >-> Sortclass.
 Arguments ContextT {_ _ _ _}, {_ _ _} _.
-Arguments lookupb {_ _ _ _} _ _ {_}, {_ _ _ _} _ _ _.
-Arguments extendb {_ _ _ _} _ _ [_] _.
+Arguments lookupb {_ _ _ _ _} _ _, {_ _ _ _} _ _ _.
+Arguments extendb {_ _ _ _} [_] _ _ _.
 Arguments removeb {_ _ _ _} _ _ _.
 Arguments empty {_ _ _ _}.
 
@@ -24,31 +24,31 @@ Section language.
 
   Local Notation flat_type := (flat_type base_type_code).
 
-  Fixpoint extend (ctx : Context) {t : flat_type}
+  Fixpoint extend {t : flat_type} (ctx : Context)
            (n : interp_flat_type (fun _ => Name) t) (v : interp_flat_type var t)
     : Context
     := match t return interp_flat_type (fun _ => Name) t -> interp_flat_type var t -> Context with
        | Tbase t => fun n v => extendb ctx n v
        | Unit => fun _ _ => ctx
        | Prod A B => fun n v
-                     => let ctx := @extend ctx A (fst n) (fst v) in
-                        let ctx := @extend ctx B (snd n) (snd v) in
+                     => let ctx := @extend A ctx (fst n) (fst v) in
+                        let ctx := @extend B ctx (snd n) (snd v) in
                         ctx
        end n v.
 
-  Fixpoint remove (ctx : Context) {t : flat_type}
+  Fixpoint remove {t : flat_type} (ctx : Context)
            (n : interp_flat_type (fun _ => Name) t)
     : Context
     := match t return interp_flat_type (fun _ => Name) t -> Context with
-       | Tbase t => fun n => removeb ctx n t
+       | Tbase t => fun n => removeb t ctx n
        | Unit => fun _ => ctx
        | Prod A B => fun n
-                     => let ctx := @remove ctx A (fst n) in
-                        let ctx := @remove ctx B (snd n) in
+                     => let ctx := @remove A ctx (fst n) in
+                        let ctx := @remove B ctx (snd n) in
                         ctx
        end n.
 
-  Definition lookup (ctx : Context) {t}
+  Definition lookup {t} (ctx : Context)
     : interp_flat_type (fun _ => Name) t -> option (interp_flat_type var t)
     := smart_interp_flat_map
          (g := fun t => option (interp_flat_type var t))
@@ -60,6 +60,6 @@ Section language.
                          end).
 End language.
 
-Global Arguments extend {_ _ _ _} ctx {_} _ _.
-Global Arguments remove {_ _ _ _} ctx {_} _.
-Global Arguments lookup {_ _ _ _} ctx {_} _, {_ _ _ _} ctx _ _.
+Global Arguments extend {_ _ _ _} {_} ctx _ _.
+Global Arguments remove {_ _ _ _} {_} ctx _.
+Global Arguments lookup {_ _ _ _} {_} ctx _, {_ _ _ _} _ ctx _.
